following suggestions

src/Collections/Sequences/Sorting.dfy
@@ -8,122 +8,17 @@
 include "../../StandardLibrary.dfy"
 include "../../UInt.dfy"
 include "../Sequences/Seq.dfy"
+include "../../Lexicographics.dfy"
 
 module Sorting {
   export
-    reveals Reflexive, AntiSymmetric, Connected, TotalOrdering
-    reveals LexicographicByteSeqBelow, LexicographicByteSeqBelowAux
-    provides AboutLexicographicByteSeqBelow
     provides SortedBy, MergeSortBy, MergeSortedBy
-    provides StandardLibrary, UInt
+    provides StandardLibrary, UInt, Lexicographics
 
   import StandardLibrary
   import opened UInt = StandardLibrary.UInt
   import opened Seq
-
-  predicate Reflexive<T(!new)>(R: (T, T) -> bool) 
-  {
-    forall x :: R(x, x)
-  }
-
-  predicate AntiSymmetric<T(!new)>(R: (T, T) -> bool) 
-  {
-    forall x, y :: R(x, y) && R(y, x) ==> x == y
-  }
-
-  predicate Connected<T(!new)>(R: (T, T) -> bool) 
-  {
-    forall x, y :: R(x, y) || R(y, x)
-  }
-
-  predicate TotalOrdering<T(!new)>(R: (T, T) -> bool) 
-  {
-    && Reflexive(R)
-    && AntiSymmetric(R)
-    && StandardLibrary.Transitive(R)
-    && Connected(R)
-  }
-
-  /*
-   * Useful orderings
-   */
-
-  // reflexivelexicographical comparison of byte sequences
-  predicate method LexicographicByteSeqBelow(x: seq<uint8>, y: seq<uint8>) 
-  {
-    LexicographicByteSeqBelowAux(x, y, 0)
-  }
-
-  predicate method LexicographicByteSeqBelowAux(x: seq<uint8>, y: seq<uint8>, n: nat)
-    requires n <= |x| && n <= |y|
-    decreases |x| - n
-  {
-    || n == |x|
-    || (n != |y| && x[n] < y[n])
-    || (n != |y| && x[n] == y[n] && LexicographicByteSeqBelowAux(x, y, n + 1))
-  }
-
-  lemma AboutLexicographicByteSeqBelow()
-    ensures TotalOrdering(LexicographicByteSeqBelow)
-  {
-    assert Reflexive(LexicographicByteSeqBelow) by {
-      forall x, n | 0 <= n <= |x| {
-        AboutLexicographicByteSeqBelowAux_Reflexive(x, n);
-      }
-    }
-    assert AntiSymmetric(LexicographicByteSeqBelow) by {
-      forall x, y, n: nat |
-        n <= |x| && n <= |y| && x[..n] == y[..n] &&
-        LexicographicByteSeqBelowAux(x, y, n) && LexicographicByteSeqBelowAux(y, x, n)
-      {
-        AboutLexicographicByteSeqBelowAux_AntiSymmetric(x, y, n);
-      }
-    }
-    assert StandardLibrary.Transitive(LexicographicByteSeqBelow) by {
-      forall x, y, z, n: nat |
-        n <= |x| && n <= |y| && n <= |z| &&
-        LexicographicByteSeqBelowAux(x, y, n) && LexicographicByteSeqBelowAux(y, z, n)
-      {
-        AboutLexicographicByteSeqBelowAux_Transitive(x, y, z, n);
-      }
-    }
-    assert Connected(LexicographicByteSeqBelow) by {
-      forall x, y, n: nat | n <= |x| && n <= |y| {
-        AboutLexicographicByteSeqBelowAux_Connected(x, y, n);
-      }
-    }
-  }
-
-  lemma AboutLexicographicByteSeqBelowAux_Reflexive(x: seq<uint8>, n: nat)
-    requires n <= |x|
-    ensures LexicographicByteSeqBelowAux(x, x, n)
-    decreases |x| - n
-  {
-  }
-
-  lemma AboutLexicographicByteSeqBelowAux_AntiSymmetric(x: seq<uint8>, y: seq<uint8>, n: nat)
-    requires n <= |x| && n <= |y|
-    requires x[..n] == y[..n]
-    requires LexicographicByteSeqBelowAux(x, y, n) && LexicographicByteSeqBelowAux(y, x, n)
-    ensures x == y
-    decreases |x| - n
-  {
-  }
-
-  lemma AboutLexicographicByteSeqBelowAux_Transitive(x: seq<uint8>, y: seq<uint8>, z: seq<uint8>, n: nat)
-    requires n <= |x| && n <= |y| && n <= |z|
-    requires LexicographicByteSeqBelowAux(x, y, n) && LexicographicByteSeqBelowAux(y, z, n)
-    ensures LexicographicByteSeqBelowAux(x, z, n)
-    decreases |x| - n
-  {
-  }
-
-  lemma AboutLexicographicByteSeqBelowAux_Connected(x: seq<uint8>, y: seq<uint8>, n: nat)
-    requires n <= |x| && n <= |y|
-    ensures LexicographicByteSeqBelowAux(x, y, n) || LexicographicByteSeqBelowAux(y, x, n)
-    decreases |x| - n
-  {
-  }
+  import opened Lexicographics
 
   predicate method SortedBy<T>(a: seq<T>,compare: (T, T) -> bool )
   {
