src/Helpers.dfy
@@ -8,128 +8,9 @@
 include "../../libraries/src/Wrappers.dfy"
 include "UInt.dfy"
 
-module StandardLibrary {
+module Helpers {
   import opened Wrappers
   import opened U = UInt
-
-  lemma SeqTakeAppend<A>(s: seq<A>, i: int)
-    requires 0 <= i < |s|
-    ensures s[..i] + [s[i]] == s[..i + 1]
-  {}
-
-  function method {:tailrecursion} Join<T>(ss: seq<seq<T>>, joiner: seq<T>): (s: seq<T>)
-    requires 0 < |ss|
-  {
-    if |ss| == 1 then ss[0] else ss[0] + joiner + Join(ss[1..], joiner)
-  }
-
-  function method {:tailrecursion} Split<T(==)>(s: seq<T>, delim: T): (res: seq<seq<T>>)
-    ensures delim !in s ==> res == [s]
-    ensures s == [] ==> res == [[]]
-    ensures 0 < |res|
-    ensures forall i :: 0 <= i < |res| ==> delim !in res[i]
-    ensures Join(res, [delim]) == s
-    decreases |s|
-  {
-    var i := FindIndexMatching(s, delim, 0);
-    if i.Some? then [s[..i.value]] + Split(s[(i.value + 1)..], delim) else [s]
-  }
-
-  lemma WillSplitOnDelim<T>(s: seq<T>, delim: T, prefix: seq<T>)
-    requires |prefix| < |s|
-    requires forall i :: 0 <= i < |prefix| ==> prefix[i] == s[i]
-    requires delim !in prefix && s[|prefix|] == delim
-    ensures Split(s, delim) == [prefix] + Split(s[|prefix| + 1..], delim)
-  {
-    calc {
-      Split(s, delim);
-    ==
-      var i := FindIndexMatching(s, delim, 0);
-      if i.Some? then [s[..i.value]] + Split(s[i.value + 1..], delim) else [s];
-    ==  { FindIndexMatchingLocatesElem(s, delim, 0, |prefix|); assert FindIndexMatching(s, delim, 0).Some?; }
-      [s[..|prefix|]] + Split(s[|prefix| + 1..], delim);
-    ==  { assert s[..|prefix|] == prefix; }
-      [prefix] + Split(s[|prefix| + 1..], delim);
-    }
-  }
-
-  lemma WillNotSplitWithOutDelim<T>(s: seq<T>, delim: T)
-    requires delim !in s
-    ensures Split(s, delim) == [s]
-  {
-    calc {
-      Split(s, delim);
-    ==
-      var i := FindIndexMatching(s, delim, 0);
-      if i.Some? then [s[..i.value]] + Split(s[i.value+1..], delim) else [s];
-    ==  { FindIndexMatchingLocatesElem(s, delim, 0, |s|); }
-      [s];
-    }
-  }
-
-  lemma FindIndexMatchingLocatesElem<T>(s: seq<T>, c: T, start: nat, elemIndex: nat)
-    requires start <= elemIndex <= |s|
-    requires forall i :: start <= i < elemIndex ==> s[i] != c
-    requires elemIndex == |s| || s[elemIndex] == c
-    ensures FindIndexMatching(s, c, start) == if elemIndex == |s| then None else Some(elemIndex)
-    decreases elemIndex - start
-    {}
-
-  function method FindIndexMatching<T(==)>(s: seq<T>, c: T, i: nat): (index: Option<nat>)
-    requires i <= |s|
-    ensures index.Some? ==>  i <= index.value < |s| && s[index.value] == c && c !in s[i..index.value]
-    ensures index.None? ==> c !in s[i..]
-    decreases |s| - i
-  {
-    FindIndex(s, x => x == c, i)
-  }
-
-  function method {:tailrecursion} FindIndex<T>(s: seq<T>, f: T -> bool, i: nat): (index: Option<nat>)
-    requires i <= |s|
-    ensures index.Some? ==> i <= index.value < |s| && f(s[index.value]) && (forall j :: i <= j < index.value ==> !f(s[j]))
-    ensures index.None? ==> forall j :: i <= j < |s| ==> !f(s[j])
-    decreases |s| - i
-  {
-    if i == |s| then None
-    else if f(s[i]) then Some(i)
-    else FindIndex(s, f, i + 1)
-  }
-
-  function method {:tailrecursion} Filter<T>(s: seq<T>, f: T -> bool): (res: seq<T>)
-    ensures forall i :: 0 <= i < |s| && f(s[i]) ==> s[i] in res
-    ensures forall i :: 0 <= i < |res| ==> res[i] in s && f(res[i])
-    ensures |res| <= |s|
-  {
-    if |s| == 0 then []
-    else if f(s[0]) then [s[0]] + Filter(s[1..], f)
-    else Filter(s[1..], f)
-  }
-
-  lemma FilterIsDistributive<T>(s: seq<T>, s': seq<T>, f: T -> bool)
-    ensures Filter(s + s', f) == Filter(s, f) + Filter(s', f)
-  {
-    if s == [] {
-      assert s + s' == s';
-    } else {
-      var S := s + s';
-      var s1 := s[1..];
-      calc {
-        Filter(S, f);
-      ==  // def. Filter
-        if f(S[0]) then [S[0]] + Filter(S[1..], f) else Filter(S[1..], f);
-      ==  { assert S[0] == s[0] && S[1..] == s1 + s'; }
-        if f(s[0]) then [s[0]] + Filter(s1 + s', f) else Filter(s1 + s', f);
-      ==  { FilterIsDistributive(s1, s', f); }
-        if f(s[0]) then [s[0]] + (Filter(s1, f) + Filter(s', f)) else Filter(s1, f) + Filter(s', f);
-      ==  // associativity of +
-        if f(s[0]) then ([s[0]] + Filter(s1, f)) + Filter(s', f) else Filter(s1, f) + Filter(s', f);
-      ==  // distribute + over if-then-else
-        (if f(s[0]) then [s[0]] + Filter(s1, f) else Filter(s1, f)) + Filter(s', f);
-      ==  // def. Filter
-        Filter(s, f) + Filter(s', f);
-      }
-    }
-  }
 
   function method Min(a: int, b: int): int {
     if a < b then a else b
@@ -412,4 +293,8 @@ module StandardLibrary {
       }
     }
   }
+}
+
+module Comparison {
+  datatype CompResult = LessThan | Equals | GreaterThan 
 }
